Prove grep_spec with 2 cheats
Lots of hacking to work around CF's poor support for higher-order
functions. I found a way to prove a custom specification for a partially
applied function, which maybe should be revisited on the original
(nicer) grep implementation.

The cheats are:
  1. regexp_matcher corresponds to regexp_lang
     This should have been proved as part of the regexp matching theory,
     but does not seem to be packaged up nicely.
  2. termination of the regexp matching algorithm. if we do not prove
     termination, then this will need to bubble up into the
     specification somehow.

characteristic/examples/grepProgScript.sml
@@ -36,6 +36,109 @@ val _ = translate(word_bit_test |> spec64);
 val _ = translate (charsetTheory.charset_full_def |> CONV_RULE (RHS_CONV EVAL));
 val _ = translate charset_mem_def;
 
+val _ = register_type``:regexp``;
+
+(* TODO: this is largely copied from the bootstrap translation
+         can it be properly abstracted out? *)
+local
+  val ths = ml_translatorLib.eq_lemmas();
+in
+  fun find_equality_type_thm tm =
+    first (can (C match_term tm) o rand o snd o strip_imp o concl) ths
+end
+
+val EqualityType_WORD = find_equality_type_thm``WORD``
+val EqualityType_CHARSET_CHARSET_TYPE = find_equality_type_thm``CHARSET_CHARSET_TYPE``
+  |> REWRITE_RULE[EqualityType_WORD]
+
+val REGEXP_REGEXP_TYPE_def = theorem"REGEXP_REGEXP_TYPE_def";
+val REGEXP_REGEXP_TYPE_ind = theorem"REGEXP_REGEXP_TYPE_ind";
+val no_closures_def = ml_translatorTheory.no_closures_def;
+val LIST_TYPE_def = ml_translatorTheory.LIST_TYPE_def;
+val EqualityType_def = ml_translatorTheory.EqualityType_def;
+val types_match_def = ml_translatorTheory.types_match_def;
+val ctor_same_type_def = semanticPrimitivesTheory.ctor_same_type_def;
+
+val REGEXP_REGEXP_TYPE_no_closures = Q.prove(
+  `∀a b. REGEXP_REGEXP_TYPE a b ⇒ no_closures b`,
+  ho_match_mp_tac REGEXP_REGEXP_TYPE_ind
+  \\ rw[REGEXP_REGEXP_TYPE_def]
+  \\ rw[no_closures_def]
+  \\ TRY (
+    qmatch_assum_rename_tac`LIST_TYPE _ x1 y1` >>
+    qhdtm_x_assum`LIST_TYPE`mp_tac >>
+    last_x_assum mp_tac >>
+    rpt(pop_assum kall_tac) >>
+    map_every qid_spec_tac[`y1`,`x1`] >>
+    Induct >> simp[LIST_TYPE_def,PULL_EXISTS,no_closures_def] >>
+    qx_gen_tac`p` >>
+    simp[PULL_EXISTS,no_closures_def] >>
+    rw[] >>
+    METIS_TAC[EqualityType_def] ) >>
+  metis_tac[EqualityType_CHARSET_CHARSET_TYPE,
+            EqualityType_def]);
+
+val REGEXP_REGEXP_TYPE_types_match = Q.prove(
+  `∀a b c d. REGEXP_REGEXP_TYPE a b ∧ REGEXP_REGEXP_TYPE c d ⇒ types_match b d`,
+  ho_match_mp_tac REGEXP_REGEXP_TYPE_ind \\
+  rw[REGEXP_REGEXP_TYPE_def] \\
+  Cases_on`c` \\ fs[REGEXP_REGEXP_TYPE_def,types_match_def,ctor_same_type_def] \\ rw[] \\
+  TRY (
+    qmatch_assum_rename_tac`LIST_TYPE _ x1 y1` >>
+    qhdtm_x_assum`LIST_TYPE`mp_tac >>
+    qmatch_assum_rename_tac`LIST_TYPE _ x2 y2` >>
+    qhdtm_x_assum`LIST_TYPE`mp_tac >>
+    last_x_assum mp_tac >>
+    rpt(pop_assum kall_tac) >>
+    map_every qid_spec_tac[`y2`,`x2`,`y1`,`x1`] >>
+    Induct >> simp[LIST_TYPE_def,PULL_EXISTS,types_match_def,ctor_same_type_def] >- (
+      Cases >> simp[LIST_TYPE_def,PULL_EXISTS,types_match_def,ctor_same_type_def] ) >>
+    qx_gen_tac`p` >>
+    gen_tac >> Cases >> simp[PULL_EXISTS,LIST_TYPE_def] >>
+    rw[types_match_def,ctor_same_type_def] >>
+    PROVE_TAC[EqualityType_def] ) >>
+  metis_tac[EqualityType_CHARSET_CHARSET_TYPE,
+            EqualityType_def]);
+
+val REGEXP_REGEXP_TYPE_11 = Q.prove(
+  `∀a b c d. REGEXP_REGEXP_TYPE a b ∧ REGEXP_REGEXP_TYPE c d ⇒ (a = c ⇔ b = d)`,
+  ho_match_mp_tac REGEXP_REGEXP_TYPE_ind \\
+  rw[REGEXP_REGEXP_TYPE_def] \\
+  Cases_on`c` \\ fs[REGEXP_REGEXP_TYPE_def] \\ rw[EQ_IMP_THM] \\
+  TRY (
+    qmatch_assum_rename_tac`LIST_TYPE _ x y1` >>
+    qhdtm_x_assum`LIST_TYPE`mp_tac >>
+    qmatch_assum_rename_tac`LIST_TYPE _ x y2` >>
+    qhdtm_x_assum`LIST_TYPE`mp_tac >>
+    last_x_assum mp_tac >>
+    rpt(pop_assum kall_tac) >>
+    map_every qid_spec_tac[`y2`,`y1`,`x`] >>
+    Induct >> simp[LIST_TYPE_def,PULL_EXISTS] >>
+    rw[] >>
+    metis_tac[]) >>
+  TRY (
+    qmatch_assum_rename_tac`LIST_TYPE _ x1 y` >>
+    qhdtm_x_assum`LIST_TYPE`mp_tac >>
+    qmatch_assum_rename_tac`LIST_TYPE _ x2 y` >>
+    qhdtm_x_assum`LIST_TYPE`mp_tac >>
+    last_x_assum mp_tac >>
+    rpt(pop_assum kall_tac) >>
+    map_every qid_spec_tac[`y`,`x1`,`x2`] >>
+    Induct >> simp[LIST_TYPE_def,PULL_EXISTS] >- (
+      Cases \\ rw[LIST_TYPE_def] ) \\
+    gen_tac \\ Cases \\ rw[LIST_TYPE_def] >>
+    metis_tac[]) >>
+  metis_tac[EqualityType_CHARSET_CHARSET_TYPE,
+            EqualityType_def]);
+
+val EqualityType_REGEXP_REGEXP_TYPE = Q.store_thm("EqualityType_REGEXP_REGEXP_TYPE",
+  `EqualityType REGEXP_REGEXP_TYPE`,
+  metis_tac[REGEXP_REGEXP_TYPE_no_closures,REGEXP_REGEXP_TYPE_types_match,REGEXP_REGEXP_TYPE_11,
+  EqualityType_def]);
+
+val _ = store_eq_thm EqualityType_REGEXP_REGEXP_TYPE;
+(* -- *)
+
 (* TODO: can the regexp one be avoided by using the mllist one instead? *)
 val zip_eq_zip = Q.store_thm("zip_eq_zip",
   `regexp$zip = mllist$zip`,
@@ -126,7 +229,7 @@ val regexp_matcher_with_limit_sound = Q.store_thm("regexp_matcher_with_limit_sou
   >> IMP_RES_TAC compile_regexp_with_limit_sound
   >> rw[pairTheory.ELIM_UNCURRY]);
 
-val _ = translate (regexp_matcher_with_limit_def);
+val r = translate (regexp_matcher_with_limit_def);
 
 val mem_tolist = Q.prove(`MEM (toList l) (MAP toList ll) = MEM l ll`,
   Induct_on `ll` >> fs[]);
@@ -1036,11 +1139,44 @@ val parse_failure_string_def = Define`
 
 val r = translate parse_failure_string_def;
 
+(* TODO: This approach (with matcher argument as a function) does not play nicely with CF
 val match_line_def = Define`
   match_line matcher (line:string) =
   case matcher line of | SOME T => T | _ => F`;
 
 val r = translate match_line_def;
+*)
+val match_line_def = Define`
+  match_line r s =
+    case regexp_matcher_with_limit r s of | SOME T => T | _ => F`;
+
+val r = translate match_line_def;
+
+val build_matcher_def = Define`
+  build_matcher r s =
+    if strlen s = 0 then
+      match_line r []
+    else
+      match_line r (FRONT (explode s))`;
+
+val r = translate build_matcher_def;
+
+val build_matcher_side = Q.prove(
+  `∀r s. build_matcher_side r s = T`,
+  rw[definition"build_matcher_side_def"]
+  \\ Cases_on`s` \\ fs[LENGTH_NIL]) |> update_precondition;
+
+val build_matcher_v_thm = theorem"build_matcher_v_thm"
+
+val build_matcher_partial_spec = Q.store_thm("build_matcher_partial_spec",
+  `REGEXP_REGEXP_TYPE r rv ⇒
+   app (p:'ffi ffi_proj) ^(fetch_v"build_matcher"(get_ml_prog_state())) [rv] emp
+    (POSTv v. &(STRING_TYPE --> BOOL) (build_matcher r) v)`,
+  strip_tac
+  \\ rw[app_def]
+  \\ irule Arrow_IMP_app_basic
+  \\ instantiate
+  \\ simp[build_matcher_v_thm]);
 
 val grep = process_topdecs`
   fun grep u =
@@ -1051,17 +1187,17 @@ val grep = process_topdecs`
        case parse_regexp (String.explode regexp) of
          NONE => print (parse_failure_string regexp)
        | SOME r =>
+           (* abandoning this approach for now ...
          let
-           (* TODO: this would be nicer as
-           val raw_match = match_line (regexp_matcher_with_limit r) s
-           but does CF support it? *)
-           fun raw_match s = match_line (fn s => regexp_matcher_with_limit r s) s
-           fun matcher s =
-             if String.strlen s = 0 then
-               raw_match []
-             else
-               raw_match (List.front (String.explode s))
-         in List.app (print_matching_lines_in_file matcher) files end`;
+           (* TODO: this would be nicer as:
+           val raw_match = match_line (regexp_matcher_with_limit r)
+             but how does partial application work in CF? *)
+           val raw_match = (fn s => match_line (fn s => regexp_matcher_with_limit r s) s)
+         in
+           *)
+           (* TODO: similar issue with higher-order function, CF seems to need this eta  *)
+           List.app (fn file => print_matching_lines_in_file (build_matcher r) file) files
+         (* end *)`;
 val _ = append_prog grep;
 
 val grep_sem_file_def = Define`
@@ -1080,5 +1216,155 @@ val grep_sem_def = Define`
    | NONE => explode (parse_failure_string (implode regexp))
    | SOME r => CONCAT (MAP (grep_sem_file (regexp_lang r) fs) (MAP implode filenames))) ∧
   (grep_sem _ _ = explode usage_string)`;
+
+val grep_spec = Q.store_thm("grep_spec",
+  `cl ≠ [] ∧ EVERY validArg cl ∧ LENGTH (FLAT cl) + LENGTH cl ≤ 256 ∧
+   CARD (set (MAP FST fs.infds)) < 255
+   ⇒
+   app (p:'ffi ffi_proj) ^(fetch_v"grep"(get_ml_prog_state()))
+    [Conv NONE []]
+    (STDOUT out * COMMANDLINE cl * ROFS fs)
+    (POSTv v. &UNIT_TYPE () v *
+      (STDOUT (out ++ grep_sem cl fs)
+       * (COMMANDLINE cl * ROFS fs)))`,
+  strip_tac
+  \\ xcf"grep"(get_ml_prog_state())
+  \\ xlet`POSTv v. &UNIT_TYPE () v * STDOUT out * COMMANDLINE cl * ROFS fs`
+  >- (xcon \\ xsimpl)
+  \\ xlet`POSTv v. &LIST_TYPE STRING_TYPE (TL (MAP implode cl)) v * STDOUT out * COMMANDLINE cl * ROFS fs`
+  >- (xapp \\ instantiate \\ xsimpl
+      \\ simp[MAP_TL,NULL_EQ,LENGTH_FLAT,MAP_MAP_o,o_DEF] (* TODO: this is duplicated in catProg and bootstrap *)
+      \\ Q.ISPECL_THEN[`STRLEN`]mp_tac SUM_MAP_PLUS
+      \\ disch_then(qspecl_then[`K 1`,`cl`]mp_tac)
+      \\ simp[MAP_K_REPLICATE,SUM_REPLICATE,GSYM LENGTH_FLAT])
+  \\ Cases_on`cl` \\ fs[]
+  \\ Cases_on`t` \\ fs[ml_translatorTheory.LIST_TYPE_def]
+  >- (
+    xmatch
+    \\ xapp
+    \\ simp[grep_sem_def]
+    \\ xsimpl
+    \\ CONV_TAC SWAP_EXISTS_CONV
+    \\ qexists_tac`usage_string`
+    \\ simp[usage_string_v_thm]
+    \\ CONV_TAC SWAP_EXISTS_CONV
+    \\ qexists_tac`out`
+    \\ xsimpl )
+  \\ rveq
+  \\ rename1`EVERY validArg t`
+  \\ Cases_on`t` \\ fs[ml_translatorTheory.LIST_TYPE_def]
+  >- (
+    xmatch
+    \\ xapp
+    \\ simp[grep_sem_def]
+    \\ xsimpl
+    \\ CONV_TAC SWAP_EXISTS_CONV
+    \\ qexists_tac`usage_string`
+    \\ simp[usage_string_v_thm]
+    \\ CONV_TAC SWAP_EXISTS_CONV
+    \\ qexists_tac`out`
+    \\ xsimpl )
+  \\ rveq
+  \\ xmatch
+  \\ rename1`grep_sem (grep::regexp::file1::files)`
+  \\ simp[grep_sem_def,MAP_MAP_o,o_DEF]
+  \\ qmatch_goalsub_abbrev_tac`COMMANDLINE cl`
+  \\ qmatch_assum_abbrev_tac`Abbrev(cl = grep::regexp::fls)`
+  \\ xlet`POSTv v. &LIST_TYPE CHAR regexp v * STDOUT out * COMMANDLINE cl * ROFS fs`
+  >- (
+    xapp
+    \\ instantiate
+    \\ simp[mlstringTheory.explode_implode]
+    \\ xsimpl )
+  \\ xlet`POSTv v. &OPTION_TYPE REGEXP_REGEXP_TYPE  (parse_regexp regexp) v * STDOUT out * COMMANDLINE cl * ROFS fs`
+  >- ( xapp \\ instantiate \\ xsimpl )
+  \\ Cases_on`parse_regexp regexp` \\ fs[ml_translatorTheory.OPTION_TYPE_def]
+  >- (
+    xmatch
+    \\ xlet`POSTv v. &STRING_TYPE (parse_failure_string (implode regexp)) v * STDOUT out * COMMANDLINE cl * ROFS fs`
+    >- (xapp \\ instantiate \\ xsimpl )
+    \\ xapp
+    \\ instantiate
+    \\ xsimpl
+    \\ CONV_TAC SWAP_EXISTS_CONV
+    \\ qexists_tac`out`
+    \\ xsimpl )
+  \\ qmatch_goalsub_abbrev_tac`gs1 ++ (FLAT (MAP ff files))`
+  \\ `gs1 ++ (FLAT (MAP ff files)) = out ++ FLAT (MAP ff fls)`
+  by ( unabbrev_all_tac \\ simp[] )
+  \\ pop_assum SUBST1_TAC
+  \\ simp[Abbr`gs1`,Abbr`ff`]
+  \\ xmatch
+  \\ rename1`parse_regexp regexp = SOME r`
+  \\ xfun_spec`appthis`
+     `∀f fv outp.
+      FILENAME f fv ∧ CARD (FDOM (alist_to_fmap fs.infds)) < 255 ⇒
+      app p appthis [fv] (STDOUT outp * COMMANDLINE cl * ROFS fs)
+        (POSTv v. &UNIT_TYPE () v * STDOUT (outp ++ grep_sem_file (regexp_lang r) fs f) * COMMANDLINE cl * ROFS fs)`
+  >- (
+    rw[]
+    \\ first_x_assum match_mp_tac
+    \\ xlet`POSTv mv. &(STRING_TYPE --> BOOL) (build_matcher r) mv * STDOUT outp * COMMANDLINE cl * ROFS fs`
+    >- ( xapp_spec build_matcher_partial_spec \\ instantiate \\ xsimpl )
+    \\ xapp
+    \\ simp[]
+    \\ instantiate
+    \\ xsimpl
+    \\ CONV_TAC SWAP_EXISTS_CONV
+    \\ qexists_tac`outp`
+    \\ xsimpl
+    \\ simp[grep_sem_file_def]
+    \\ reverse IF_CASES_TAC
+    >- (
+      CASE_TAC \\ xsimpl
+      \\ imp_res_tac ALOOKUP_SOME_inFS_fname )
+    \\ imp_res_tac inFS_fname_ALOOKUP_EXISTS
+    \\ simp[]
+    \\ qmatch_goalsub_abbrev_tac`STDOUT (outp ++ s1)`
+    \\ qmatch_goalsub_abbrev_tac`STDOUT (outp ++ s2) * _`
+    \\ `s1 = s2` suffices_by xsimpl
+    \\ simp[Abbr`s1`,Abbr`s2`]
+    \\ AP_TERM_TAC
+    \\ simp[FILTER_MAP,MAP_MAP_o]
+    \\ simp[Once o_DEF]
+    \\ AP_TERM_TAC
+    \\ AP_THM_TAC
+    \\ AP_TERM_TAC
+    \\ simp[FUN_EQ_THM,build_matcher_def]
+    \\ simp[mlstringTheory.explode_implode]
+    \\ simp[mlstringTheory.implode_def]
+    \\ simp[FRONT_APPEND]
+    \\ simp[match_line_def]
+    \\ gen_tac
+    \\ TOP_CASE_TAC
+    >- cheat (* false : this is because of the termination proof. grep_sem will need to be uglified to accommodate this *)
+    \\ imp_res_tac regexp_matcher_with_limit_sound
+    \\ rveq
+    \\ cheat (* this should be proved separately as a top-level theorem about regexp_matcher *) )
+  \\ xapp_spec (INST_TYPE[alpha|->``:mlstring``]mllistProgTheory.app_spec)
+  \\ CONV_TAC (RESORT_EXISTS_CONV List.rev)
+  \\ qexists_tac`λn. STDOUT (out ++ (CONCAT (MAP (grep_sem_file (regexp_lang r) fs) (TAKE n (MAP implode fls))))) * COMMANDLINE cl * ROFS fs`
+  \\ xsimpl
+  \\ qexists_tac`MAP implode fls`
+  \\ qexists_tac`STRING_TYPE`
+  \\ reverse conj_tac
+  >- ( simp[Abbr`fls`,MAP_MAP_o,o_DEF] \\ xsimpl )
+  \\ reverse conj_tac
+  >- ( simp[Abbr`fls`,ml_translatorTheory.LIST_TYPE_def] )
+  \\ rw[] \\ rfs[EL_MAP]
+  \\ qmatch_assum_abbrev_tac`STRING_TYPE f xv`
+  \\ `validArg (explode f)`
+  by (
+    fs[Abbr`fls`,Abbr`f`,mlstringTheory.explode_implode,EVERY_MEM,MEM_EL,PULL_EXISTS]
+    \\ Cases_on`n` \\ fs[] )
+  \\ `FILENAME f xv`
+  by (
+    fs[FILENAME_def,commandLineFFITheory.validArg_def,Abbr`f`,mlstringTheory.explode_implode,mlstringTheory.implode_def]
+    \\ fs[EVERY_MEM] )
+  \\ first_x_assum drule
+  \\ `TAKE (n+1) fls = (TAKE n fls) ++ [EL n fls]` by ( simp[TAKE_EL_SNOC] )
+  \\ simp[GSYM MAP_TAKE]
+  \\ simp[MAP_MAP_o]
+  \\ simp[set_sepTheory.STAR_ASSOC]);
 
 val _ = export_theory ();
